got recusrive encode/decode working!

simrec.bpl
@@ -24,8 +24,16 @@ function get_hi_range(sym: int, range: int) returns(int);
 axiom (forall i,r: int :: {get_hi_range(i,r)} get_hi_range(i,r)<=r && get_lo_range(i,r) < get_hi_range(i,r));
 
 function lookup(x: int, range: int) returns(int);
-axiom (forall x,r: int :: {lookup(x,r)} x>=0 && x<r ==> x<=get_lo_range(lookup(x,r), r) && x<get_hi_range(lookup(x,r), r));
+//pre? x>=0 && x<r ==> 
+//axiom (forall x,r: int :: {lookup(x,r)} x>=get_lo_range(lookup(x,r), r) && x<get_hi_range(lookup(x,r), r));
+axiom (forall x,r,y: int :: y==lookup(x,r) <==> x>=get_lo_range(y, r) && x<get_hi_range(y, r));
 
+function encodef(ind: int, range: int) returns (int);
+axiom (forall i,r: int :: {encodef(i, r)} i>=len ==> encodef(i, r) == 0);
+axiom (forall i,r: int :: {encodef(i, r)} i>=0 && i<len ==> encodef(i, r) == get_lo_range(in[i], r)+encodef(i+1, get_hi_range(in[i], r)-get_lo_range(in[i], r)));
+
+//TODO
+axiom (forall i,r: int :: {encodef(i, r)} i>=0 && i<len ==> encodef(i, r) >= get_lo_range(in[i], r) && encodef(i, r) < get_hi_range(in[i], r));
 
 procedure encode(ind: int, range: int) returns (x: int)
     requires len>=0;
@@ -33,8 +41,10 @@ procedure encode(ind: int, range: int) returns (x: int)
     requires (forall i: int :: i>=0 && i<len ==> in[i]>=0 && in[i]<nsyms);
     //requires range>0;
     ensures x>=0 && x<range;
+    ensures ind>=len ==> x==0;
     ensures ind<len ==> x>=get_lo_range(in[ind], range) && x<get_hi_range(in[ind], range);
     //ensures x in the range that makes out[i]==in[i], recursive call
+    ensures x == encodef(ind, range);
 {
     var c, lo, hi: int;
     assume (range > 0); // TODO
@@ -54,16 +64,18 @@ procedure decode(ind: int, range: int, x: int)
     requires ind>=0 && ind<=len;
     requires range>0;
 //    ensures that gets first letter right and returns decode(1..)
-    ensures (forall i: int :: i>=ind && i<len ==> out[i]==in[i]);
+    ensures ((x==encodef(ind, range)) ==> (forall i: int :: i>=ind && i<len ==> out[i]==in[i]));
+    //ensures x==encodef(ind, range) && ind<len ==> out[ind]==in[ind];
 {
     var c, lo, hi: int;
     assume (range > 0); // TODO
     if (ind>=len) { return; }
     c := lookup(x, range);
-    assume (c == in[ind]); //TODO this is cheating
+    //assert(x == encodef(ind, range) ==> c==in[ind]);
+    //assume (c == in[ind]); //TODO this is cheating
     lo := get_lo_range(c, range);
     hi := get_hi_range(c, range);
-    assume (x>=lo); // TODO
+    //assume (x>=lo); // TODO
     call decode(ind+1, hi-lo, x-lo);
     out[ind] := c;
 }
@@ -73,6 +85,9 @@ procedure main() modifies out; {
     var range: int where range>0; //TODO calc range
        
     call x := encode(0, range);
+    
+    //assume(x >= 0 && x<range);
+    
     call decode(0, range, x);
     assert (forall i: int :: i>=0 && i<len ==> out[i]==in[i]);
 }
